theory/x64EncodeProof.thy
@@ -1,0 +1,13 @@
+theory x64EncodeProof
+imports
+  Main
+  rBPFCommType rBPFSyntax
+  x64Assembler x64Disassembler
+begin
+lemma x64_decode_encode_consistency:
+  "x64_decode pc l = Some (length l_bin, ins) \<Longrightarrow> (Some l_bin = x64_encode ins \<and> list_in_list l_bin pc l)"
+  apply (cases ins; simp_all)
+
+  done
+
+end
